{
 "cells": [
  {
   "cell_type": "markdown",
   "metadata": {},
   "source": [
    "## Computing $b^{\\mu}$ and $S^i$, using [Duez *et al* (2005)](https://arxiv.org/pdf/astro-ph/0503420.pdf)\n",
    "\n",
    "First some definitions. The spatial components of $b^{\\mu}$ are simply the magnetic field as measured by an observer comoving with the plasma $B^{\\mu}_{\\rm (u)}$, divided by $\\sqrt{4\\pi}$. In addition, in the ideal MHD limit, $B^{\\mu}_{\\rm (u)}$ is orthogonal to the plasma 4-velocity $u^\\mu$, which sets the $\\mu=0$ component. \n",
    "\n",
    "Note also that $B^{\\mu}_{\\rm (u)}$ is related to the magnetic field as measured by a *normal* observer $B^i$ via a simple projection (Eq 21 in Duez et al), which results in the expressions (Eqs 23 and 24 in Duez et al):\n",
    "\n",
    "\\begin{align}\n",
    "\\sqrt{4\\pi} b^0 = B^0_{\\rm (u)} &= \\frac{u_j B^j}{\\alpha} \\\\\n",
    "\\sqrt{4\\pi} b^i = B^i_{\\rm (u)} &= \\frac{B^i + (u_j B^j) u^i}{\\alpha u^0}\\\\\n",
    "\\end{align}\n",
    "\n",
    "$B^i$ is related to the actual magnetic field evaluated in IllinoisGRMHD, $\\tilde{B}^i$ via\n",
    "\n",
    "$$B^i = \\frac{\\tilde{B}^i}{\\gamma},$$\n",
    "\n",
    "where $\\gamma$ is the determinant of the spatial 3-metric.\n",
    "\n",
    "The above expressions will require that we compute\n",
    "1. the 4-metric $g_{\\mu\\nu}$ from the ADM 3+1 variables\n",
    "1. $u^0$ from the Valencia 3-velocity\n",
    "1. $u_j$ from $u^0$, the Valencia 3-velocity, and $g_{\\mu\\nu}$\n",
    "1. $\\gamma$ from the ADM 3+1 variables\n",
    "\n",
    "## Step 1: Compute the 4-metric $g_{\\mu\\nu}$ from the ADM 3+1 variables\n",
    "We are given $\\gamma_{ij}$, $\\alpha$, and $\\beta^i$ from ADMBase, so let's first compute \n",
    "\n",
    "$$\n",
    "g_{\\mu\\nu} = \\begin{pmatrix} \n",
    "-\\alpha^2 + \\beta^k \\beta_k & \\beta_i \\\\\n",
    "\\beta_j & \\gamma_{ij}\n",
    "\\end{pmatrix}.\n",
    "$$"
   ]
  },
  {
   "cell_type": "code",
   "execution_count": 1,
   "metadata": {},
   "outputs": [],
   "source": [
    "import sympy as sp\n",
    "import NRPy_param_funcs as par\n",
    "import grid as gri\n",
    "import indexedexp as ixp\n",
    "import reference_metric as rfm\n",
    "\n",
    "# Set spatial dimension = 3\n",
    "DIM=3\n",
    "\n",
    "gammaDD = ixp.register_gridfunctions_for_single_rank2(\"AUX\",\"gammaDD\", \"sym01\",DIM=3)\n",
    "betaU   = ixp.register_gridfunctions_for_single_rank1(\"AUX\",\"betaU\",DIM=3)\n",
    "alpha   = gri.register_gridfunctions(\"AUX\",\"alpha\")\n",
    "\n",
    "# To get \\gamma_{\\mu \\nu} = gammabar4DD[mu][nu], we'll need to construct the 4-metric, using Eq. 2.122 in B&S:\n",
    "g4DD = ixp.zerorank2(DIM=4)\n",
    "\n",
    "# Eq. 2.121 in B&S\n",
    "betaD = ixp.zerorank1()\n",
    "for i in range(DIM):\n",
    "    for j in range(DIM):\n",
    "        betaD[i] += gammaDD[i][j]*betaU[j]\n",
    "\n",
    "# Now compute the beta contraction.\n",
    "beta2 = sp.sympify(0)\n",
    "for i in range(DIM):\n",
    "    beta2 += betaU[i]*betaD[i]\n",
    "\n",
    "# Eq. 2.122 in B&S\n",
    "g4DD[0][0] = -alpha**2 + beta2\n",
    "for mu in range(1,4):\n",
    "    g4DD[mu][0] = g4DD[0][mu] = betaD[mu-1]\n",
    "for mu in range(1,4):\n",
    "    for nu in range(1,4):\n",
    "        g4DD[mu][nu] = gammaDD[mu-1][nu-1]"
   ]
  },
  {
   "cell_type": "markdown",
   "metadata": {},
   "source": [
    "## Step 2: Compute $u^0$ from the Valencia 3-velocity\n",
    "\n",
    "According to Eqs. 9-11 of [the IllinoisGRMHD paper](https://arxiv.org/pdf/1501.07276.pdf), the Valencia 3-velocity $v^i_{(n)}$ is related to the 4-velocity $u^\\mu$ via\n",
    "\n",
    "\\begin{align}\n",
    "\\alpha v^i_{(n)} &= \\frac{u^i}{u^0} + \\beta^i \\\\\n",
    "\\implies u^i &= u^0 \\left(\\alpha v^i_{(n)} - \\beta^i\\right)\n",
    "\\end{align}\n",
    "\n",
    "Defining $v^i = \\frac{u^i}{u^0}$, we get\n",
    "\n",
    "$$v^i = \\alpha v^i_{(n)} - \\beta^i,$$\n",
    "\n",
    "and in terms of this variable we get\n",
    "\n",
    "\\begin{align}\n",
    "g_{00} \\left(u^0\\right)^2 + 2 g_{0i} u^0 u^i + g_{ij} u^i u^j &= \\left(u^0\\right)^2 \\left(g_{00} + 2 g_{0i} v^i + g_{ij} v^i v^j\\right)\\\\\n",
    "\\implies u^0 &= \\sqrt{\\frac{-1}{g_{00} + 2 g_{0i} v^i + g_{ij} v^i v^j}} \\\\\n",
    "&= \\sqrt{\\frac{-1}{(-\\alpha^2 + \\beta^2) + 2 \\beta_i v^i + \\gamma_{ij} v^i v^j}} \\\\\n",
    "\\end{align}"
   ]
  },
  {
   "cell_type": "markdown",
   "metadata": {},
   "source": [
    "## Appendix: Proving Eqs. 53 and 56 in [Duez *et al* (2005)](https://arxiv.org/pdf/astro-ph/0503420.pdf)\n",
    "\n",
    "Thus $u^\\mu u_\\mu = -1$ implies\n",
    "\n",
    "\\begin{align}\n",
    "g^{\\mu\\nu} u_\\mu u_\\nu &= g^{00} \\left(u_0\\right)^2 + 2 g^{0i} u_0 u_i + g^{ij} u_i u_j = -1 \\\\\n",
    "\\implies &g^{00} \\left(u_0\\right)^2 + 2 g^{0i} u_0 u_i + g^{ij} u_i u_j + 1 = 0\\\\\n",
    "& a x^2 + b x + c = 0\n",
    "\\end{align}\n",
    "\n",
    "Thus we have a quadratic equation for $u_0$, with solution given by\n",
    "\n",
    "\\begin{align}\n",
    "u_0 &= \\frac{-b \\pm \\sqrt{b^2 - 4 a c}}{2 a} \\\\\n",
    "&= \\frac{-2 g^{0i}u_i \\pm \\sqrt{\\left(2 g^{0i} u_i\\right)^2 - 4 g^{00} (g^{ij} u_i u_j + 1)}}{2 g^{00}}\\\\\n",
    "&= \\frac{-g^{0i}u_i \\pm \\sqrt{\\left(g^{0i} u_i\\right)^2 - g^{00} (g^{ij} u_i u_j + 1)}}{g^{00}}\\\\\n",
    "\\end{align}\n",
    "\n",
    "Notice that (Eq. 4.49 in [Gourgoulhon](https://arxiv.org/pdf/gr-qc/0703035.pdf))\n",
    "$$\n",
    "g^{\\mu\\nu} = \\begin{pmatrix} \n",
    "-\\frac{1}{\\alpha^2} & \\frac{\\beta^i}{\\alpha^2} \\\\\n",
    "\\frac{\\beta^i}{\\alpha^2} & \\gamma^{ij} - \\frac{\\beta^i\\beta^j}{\\alpha^2}\n",
    "\\end{pmatrix},\n",
    "$$\n",
    "so we have\n",
    "\n",
    "\\begin{align}\n",
    "u_0 &= \\frac{-\\beta^i u_i/\\alpha^2 \\pm \\sqrt{\\left(\\beta^i u_i/\\alpha^2\\right)^2 + 1/\\alpha^2 (g^{ij} u_i u_j + 1)}}{1/\\alpha^2}\\\\\n",
    "&= -\\beta^i u_i \\pm \\sqrt{\\left(\\beta^i u_i\\right)^2 + \\alpha^2 (g^{ij} u_i u_j + 1)}\\\\\n",
    "&= -\\beta^i u_i \\pm \\sqrt{\\left(\\beta^i u_i\\right)^2 + \\alpha^2 \\left(\\left[\\gamma^{ij} - \\frac{\\beta^i\\beta^j}{\\alpha^2}\\right] u_i u_j + 1\\right)}\\\\\n",
    "&= -\\beta^i u_i \\pm \\sqrt{\\left(\\beta^i u_i\\right)^2 + \\alpha^2 \\left(\\gamma^{ij}u_i u_j + 1\\right) - \\beta^i\\beta^j u_i u_j}\\\\\n",
    "&= -\\beta^i u_i \\pm \\sqrt{\\alpha^2 \\left(\\gamma^{ij}u_i u_j + 1\\right)}\\\\\n",
    "\\end{align}\n",
    "\n",
    "Now, since \n",
    "\n",
    "$$\n",
    "u^0 = g^{\\alpha 0} u_\\alpha = -\\frac{1}{\\alpha^2} u_0 + \\frac{\\beta^i u_i}{\\alpha^2},\n",
    "$$\n",
    "\n",
    "we get\n",
    "\n",
    "\\begin{align}\n",
    "u^0 &= \\frac{1}{\\alpha^2} \\left(u_0 + \\beta^i u_i\\right) \\\\\n",
    "&= \\pm \\frac{1}{\\alpha^2} \\sqrt{\\alpha^2 \\left(\\gamma^{ij}u_i u_j + 1\\right)}\\\\\n",
    "&= \\pm \\frac{1}{\\alpha} \\sqrt{\\gamma^{ij}u_i u_j + 1}\\\\\n",
    "\\end{align}\n",
    "\n",
    "By convention, the relativistic Gamma factor is positive and given by $\\alpha u^0$, so we choose the positive root. Thus we have derived Eq. 53 in [Duez *et al* (2005)](https://arxiv.org/pdf/astro-ph/0503420.pdf):\n",
    "\n",
    "$$\n",
    "u^0 = \\frac{1}{\\alpha} \\sqrt{\\gamma^{ij}u_i u_j + 1}.\n",
    "$$\n",
    "\n",
    "Next we evaluate \n",
    "\n",
    "\\begin{align}\n",
    "u^i &= u_\\mu g^{\\mu i} \\\\\n",
    "&= u_0 g^{0 i} + u_j g^{i j}\\\\\n",
    "&= u_0 \\frac{\\beta^i}{\\alpha^2} + u_j \\left(\\gamma^{ij} - \\frac{\\beta^i\\beta^j}{\\alpha^2}\\right)\\\\\n",
    "&= \\gamma^{ij} u_j + u_0 \\frac{\\beta^i}{\\alpha^2} - u_j \\frac{\\beta^i\\beta^j}{\\alpha^2}\\\\\n",
    "&= \\gamma^{ij} u_j + \\frac{\\beta^i}{\\alpha^2} \\left(u_0  - u_j \\beta^j\\right)\\\\\n",
    "&= \\gamma^{ij} u_j - \\beta^i u^0,\n",
    "\\end{align}\n",
    "\n",
    "which is equivalent to Eq. 56 in [Duez *et al* (2005)](https://arxiv.org/pdf/astro-ph/0503420.pdf). Notice in the last step, we used the above definition of $u^0$."
   ]
  }
 ],
 "metadata": {
  "kernelspec": {
   "display_name": "Python 3",
   "language": "python",
   "name": "python3"
  },
  "language_info": {
   "codemirror_mode": {
    "name": "ipython",
    "version": 3
   },
   "file_extension": ".py",
   "mimetype": "text/x-python",
   "name": "python",
   "nbconvert_exporter": "python",
   "pygments_lexer": "ipython3",
   "version": "3.6.6"
  }
 },
 "nbformat": 4,
 "nbformat_minor": 2
}
